TouhouFormal/ECL.lean
@@ -41,4 +41,5 @@ import TouhouFormal.ECL.Extension
 import TouhouFormal.ECL.ChildContext
 import TouhouFormal.ECL.Misc
 import TouhouFormal.ECL.BossDispatch
+import TouhouFormal.ECL.LinkedChild
 import TouhouFormal.ECL.Boss
